$case \ 1: n \neq m$

$$
\begin{align*}
\begin{gather*}
\int{sin(mt)sin(nt)}dt =\frac{1}{2} \int{cos(t(n-m)) - cos(t(n+m))}dt \\
= \frac{sin(t(n-m))}{2(n-m)} - \frac{sin(t(n+m))}{2(n+m)} + C
\end{gather*}
\end{align*}
$$

$$
\begin{align*}
\begin{gather*}
\int{cos(mt)cos(nt)}dt =\frac{1}{2} \int{cos(t(n-m)) + cos(t(n+m))}dt \\
= \frac{sin(t(n-m))}{2(n-m)} + \frac{sin(t(n+m))}{2(n+m)} + C
\end{gather*}
\end{align*}
$$

$case \ 2: n = m$

$$
\begin{align*}
\begin{gather*}
\int{sin^2{(nt)}}dt =\frac{1}{2} \int{1-cos{(2nt)}}dt \\
=\frac{t}{2} -\frac{1}{4n}sin(2nt) + C
\end{gather*}
\end{align*}
$$

$$
\begin{align*}
\begin{gather*}
\int{cos^2{(nt)}}dt =\frac{1}{2} \int{cos{(2nt)+1}}dt \\
= \frac{1}{4n}sin(2nt) + \frac{t}{2} + C
\end{gather*}
\end{align*}
$$
